code/ecdsap256/Hacl.Impl.P256.Arithmetics.fsti
@@ -21,6 +21,7 @@ open FStar.Math.Lemmas
 
 open FStar.Mul
 
+inline_for_extraction noextract
 val cube: a: felem -> result: felem -> Stack unit
   (requires fun h -> live h a /\ live h result /\ disjoint a result /\ as_nat h a < prime)
   (ensures fun h0 _ h1 -> modifies (loc result) h0 h1 /\ 
@@ -35,6 +36,7 @@ val quatre: a: felem -> result: felem -> Stack unit
     as_nat h1 result = toDomain_ (fromDomain_ (as_nat h0 a) * fromDomain_ (as_nat h0 a) * fromDomain_ (as_nat h0 a) * fromDomain_ (as_nat h0 a) % prime256) /\ 
     as_nat h1 result = toDomain_ (fromDomain_ (as_nat h0 a) * fromDomain_ (as_nat h0 a) * fromDomain_ (as_nat h0 a) * fromDomain_ (as_nat h0 a)))
 
+inline_for_extraction noextract
 val multByTwo: a: felem -> result: felem -> Stack unit 
   (requires fun h -> live h a /\ live h result /\ eq_or_disjoint a result /\ as_nat h a < prime )
   (ensures fun h0 _ h1 -> modifies (loc result) h0 h1 /\ 
@@ -42,6 +44,7 @@ val multByTwo: a: felem -> result: felem -> Stack unit
     as_nat h1 result == toDomain_ (2 * fromDomain_ (as_nat h0 a)) /\ 
     as_nat h1 result < prime)
 
+inline_for_extraction noextract
 val multByThree: a: felem -> result: felem -> Stack unit 
   (requires fun h -> live h a /\ live h result /\ disjoint a result /\ as_nat h a < prime )
   (ensures fun h0 _ h1 -> modifies (loc result) h0 h1 /\ as_nat h1 result < prime /\ 
@@ -49,7 +52,7 @@ val multByThree: a: felem -> result: felem -> Stack unit
     as_nat h1 result == toDomain_ (3 * fromDomain_ (as_nat h0 a))
   )
 
-
+inline_for_extraction noextract
 val multByFour: a: felem -> result: felem -> Stack unit 
   (requires fun h -> live h a /\ live h result /\ eq_or_disjoint a result /\ as_nat h a < prime )
   (ensures fun h0 _ h1 -> modifies (loc result) h0 h1 /\ as_nat h1 result < prime /\ 
@@ -57,6 +60,7 @@ val multByFour: a: felem -> result: felem -> Stack unit
     as_nat h1 result == toDomain_ (4 * fromDomain_ (as_nat h0 a))
 )
 
+inline_for_extraction noextract
 val multByEight: a: felem -> result: felem -> Stack unit 
   (requires fun h -> live h a /\ live h result /\ disjoint a result /\ as_nat h a < prime )
   (ensures fun h0 _ h1 -> modifies (loc result) h0 h1 /\ as_nat h1 result < prime /\ 
@@ -64,6 +68,7 @@ val multByEight: a: felem -> result: felem -> Stack unit
     as_nat h1 result == toDomain_ (8 * fromDomain_ (as_nat h0 a))
 )
 
+inline_for_extraction noextract
 val multByMinusThree: a: felem -> result: felem -> Stack unit 
   (requires fun h -> live h a /\ live h result /\ disjoint a result /\ as_nat h a < prime )
   (ensures fun h0 _ h1 -> modifies (loc result) h0 h1 /\ 
