code/ecdsap256/Hacl.Impl.P256.Primitives.fst
@@ -1,0 +1,296 @@
+module Hacl.Impl.P256.Primitives
+
+open FStar.HyperStack.All
+open FStar.HyperStack
+module ST = FStar.HyperStack.ST
+
+open Lib.IntTypes
+open Lib.Buffer
+open Lib.ByteSequence
+
+open Spec.P256
+open Spec.ECDSA
+open Spec.P256.Definitions
+open Spec.DH
+open Spec.ECDSAP256.Definition
+open Spec.P256.Lemmas
+
+open Hacl.Impl.P256.LowLevel 
+open Hacl.Impl.P256.Core
+open Hacl.Impl.P256.Signature.Common
+
+#set-options "--fuel 0 --ifuel 0 --z3rlimit 200"
+
+inline_for_extraction noextract
+val _toForm: i:lbuffer uint8 (size 32) -> o:felem -> Stack unit
+  (requires fun h -> live h i /\ live h o /\ disjoint i o)
+  (ensures  fun h0 _ h1 ->
+    modifies (loc o) h0 h1 /\ as_nat h1 o == nat_from_bytes_be (as_seq h0 i))
+
+let _toForm i o = 
+    let h0 = ST.get() in 
+  toUint64ChangeEndian i o;
+    let h1 = ST.get() in 
+  changeEndianLemma (uints_from_bytes_be (as_seq h0 i));
+  uints_from_bytes_be_nat_lemma #U64 #_ #4 (as_seq h0 i);
+  lemma_core_0 o h1
+
+
+val toFormPoint: i: lbuffer uint8 (size 64) -> result: point -> Stack unit 
+  (requires fun h -> live h i /\ live h result /\ disjoint i result)
+  (ensures fun h0 _ h1 -> modifies (loc result) h0 h1 /\ (
+    let pointScalarXSeq = nat_from_bytes_be (as_seq h0 (gsub i (size 0) (size 32))) in 
+    let pointScalarYSeq = nat_from_bytes_be (as_seq h0 (gsub i (size 32) (size 32))) in 
+    let x, y, z = point_prime_to_coordinates (as_seq h1 result) in 
+    let pointJacX, pointJacY, pointJacZ = toJacobianCoordinates (pointScalarXSeq, pointScalarYSeq) in 
+    x == pointScalarXSeq /\ y == pointScalarYSeq /\ z == 1 /\
+    x == pointJacX /\ y == pointJacY /\ z == pointJacZ))
+
+      
+let toFormPoint i p = 
+  let pointScalarX = sub i (size 0) (size 32) in 
+  let pointScalarY = sub i (size 32) (size 32) in 
+
+  let pointX = sub p (size 0) (size 4) in 
+  let pointY = sub p (size 4) (size 4) in 
+  let pointZ = sub p (size 8) (size 4) in 
+
+  _toForm pointScalarX pointX;
+  _toForm pointScalarY pointY;
+  uploadOneImpl pointZ
+
+
+inline_for_extraction noextract
+val _fromForm: i: felem -> o: lbuffer uint8 (size 32) -> Stack unit 
+  (requires fun h -> live h i /\ live h o /\ disjoint i o /\ as_nat h i < pow2 256)
+  (ensures fun h0 _ h1 -> modifies (loc i |+| loc o) h0 h1 /\  as_seq h1 o == nat_to_bytes_be 32  (as_nat h0 i))
+
+let _fromForm i o = 
+    let h0 = ST.get() in 
+  changeEndian i;
+  toUint8 i o;
+  
+  lemma_core_0 i h0;
+  lemma_nat_from_to_intseq_le_preserves_value 4 (as_seq h0 i);
+  changeEndian_le_be (as_nat h0 i)
+
+
+val fromFormPoint: i: point -> o: lbuffer uint8 (size 64) -> Stack unit
+  (requires fun h -> live h i /\ live h o /\ disjoint i o /\
+    as_nat h (gsub i (size 0) (size 4)) < prime256 /\
+    as_nat h (gsub i (size 4) (size 4)) < prime256 )
+  (ensures fun h0 _ h1 -> modifies (loc i |+| loc o) h0 h1 /\ (
+    let xCoordinate = gsub i (size 0) (size 4) in 
+    let yCoordinate = gsub i (size 4) (size 4) in 
+
+    let scalarX = gsub o (size 0) (size 32) in 
+    let scalarY = gsub o (size 32) (size 32) in 
+
+    as_seq h1 scalarX == nat_to_bytes_be 32 (as_nat h0 xCoordinate) /\
+    as_seq h1 scalarY == nat_to_bytes_be 32 (as_nat h0 yCoordinate)))
+
+
+let fromFormPoint i o = 
+  let pointX = sub i (size 0) (size 4) in 
+  let pointY = sub i (size 4) (size 4) in 
+
+  let pointScalarX = sub o (size 0) (size 32) in 
+  let pointScalarY = sub o (size 32) (size 32) in 
+
+  _fromForm pointX pointScalarX;
+  _fromForm pointY pointScalarY
+
+
+
+
+inline_for_extraction noextract
+val secretToPublic:
+    result:lbuffer uint8 (size 64)
+  -> scalar:lbuffer uint8 (size 32)
+  -> Stack bool
+  (requires fun h ->
+    live h result /\ live h scalar /\ 
+    disjoint result scalar)
+  (ensures fun h0 r h1 ->
+    let pointX, pointY, flag = ecp256_dh_i (as_seq h0 scalar) in
+    modifies (loc result) h0 h1 /\
+    r == flag /\
+    as_seq h1 (gsub result (size 0) (size 32)) == pointX /\
+    as_seq h1 (gsub result (size 32) (size 32)) == pointY)
+    
+
+let secretToPublic result scalar = 
+    push_frame();
+  let tempBuffer = create (size 100) (u64 0) in
+  let resultBuffer = create (size 12) (u64 0) in
+  
+  secretToPublic resultBuffer scalar tempBuffer;
+  let flag = isPointAtInfinityPrivate resultBuffer in
+  fromFormPoint resultBuffer result;
+  
+  pop_frame();
+
+  let open Hacl.Impl.P256.LowLevel.RawCmp in 
+  unsafe_bool_of_u64  flag
+
+
+(*
+  This function provides a raw implementation of the secrettopublic function. 
+  It doesnot provide the verification that the point gotten at the result doesnot belong to infinity.
+  We strongly discourage you to use this function unless you understand what you´re doing.
+  A. 
+*)
+
+inline_for_extraction noextract
+val secretToPublicRaw:
+    result:lbuffer uint8 (size 64)
+  -> scalar:lbuffer uint8 (size 32)
+  -> Stack unit
+  (requires fun h ->
+    live h result /\ live h scalar /\ 
+    disjoint result scalar)
+  (ensures fun h0 r h1 ->
+    modifies (loc result) h0 h1 /\ (
+    let (xN, yN, zN) = secret_to_public (as_seq h0 scalar)  in 
+
+    let scalarX = gsub result (size 0) (size 32) in 
+    let scalarY = gsub result (size 32) (size 32) in 
+
+    as_seq h1 scalarX == nat_to_bytes_be 32 xN /\
+    as_seq h1 scalarY == nat_to_bytes_be 32 yN))
+
+
+let secretToPublicRaw result scalar =
+  push_frame();
+  let tempBuffer = create (size 100) (u64 0) in
+  let resultBuffer = create (size 12) (u64 0) in
+
+  Hacl.Impl.P256.Core.secretToPublic resultBuffer scalar tempBuffer;  
+  fromFormPoint resultBuffer result;
+  pop_frame()
+
+
+inline_for_extraction noextract
+val scalarMult:
+    result:lbuffer uint8 (size 64)
+  -> pubKey:lbuffer uint8 (size 64)
+  -> scalar:lbuffer uint8 (size 32)
+  -> Stack bool
+    (requires fun h ->
+      live h result /\ live h pubKey /\ live h scalar /\
+      disjoint result pubKey /\ disjoint result scalar)
+    (ensures fun h0 r h1 ->
+      let pubKeyX = gsub pubKey (size 0) (size 32) in
+      let pubKeyY = gsub pubKey (size 32) (size 32) in
+      let pointX, pointY, flag =
+        ecp256_dh_r (as_seq h0 pubKeyX) (as_seq h0 pubKeyY) (as_seq h0 scalar) in
+      r == flag /\
+      modifies (loc result) h0 h1 /\
+      as_seq h1 (gsub result (size 0) (size 32)) == pointX /\
+      as_seq h1 (gsub result (size 32) (size 32)) == pointY)
+
+
+let scalarMult result pubKey scalar =
+  push_frame();
+  
+  let resultBufferFelem = create (size 12) (u64 0) in
+  let publicKeyAsFelem = create (size 12) (u64 0) in
+  let tempBuffer = create (size 100) (u64 0) in
+  
+  toFormPoint pubKey publicKeyAsFelem; 
+  let publicKeyCorrect = verifyQValidCurvePoint publicKeyAsFelem tempBuffer in
+  
+  let flag = 
+    if publicKeyCorrect then
+      begin
+      scalarMultiplication publicKeyAsFelem resultBufferFelem scalar tempBuffer;
+      isPointAtInfinityPrivate resultBufferFelem 
+      end
+    else 
+      u64 18446744073709551615 in 
+      
+  (* This line is a bit suspicious *)
+  fromFormPoint resultBufferFelem result;
+  
+  pop_frame();
+  
+  let open Hacl.Impl.P256.LowLevel.RawCmp in 
+  unsafe_bool_of_u64  flag
+
+
+
+inline_for_extraction noextract
+val scalarMultRaw:
+    result:lbuffer uint8 (size 64)
+  -> pubKey:lbuffer uint8 (size 64)
+  -> scalar:lbuffer uint8 (size 32)
+  -> Stack unit
+    (requires fun h ->
+      live h result /\ live h pubKey /\ live h scalar /\
+      disjoint result pubKey /\ disjoint result scalar /\ (
+      let x, y = gsub pubKey (size 0) (size 32), gsub pubKey (size 32) (size 32) in 
+      nat_from_bytes_be (as_seq h x) < prime256 /\
+      nat_from_bytes_be (as_seq h y) < prime256))
+    (ensures fun h0 _ h1 -> modifies (loc result |+| loc pubKey) h0 h1 /\ (
+      let pointScalarXSeq = nat_from_bytes_be (as_seq h0 (gsub pubKey (size 0) (size 32))) in 
+      let pointScalarYSeq = nat_from_bytes_be (as_seq h0 (gsub pubKey (size 32) (size 32))) in  
+      let pointJacX, pointJacY, pointJacZ = toJacobianCoordinates (pointScalarXSeq, pointScalarYSeq) in 
+      let (xN, yN, zN) = scalar_multiplication (as_seq h0 scalar) (pointJacX, pointJacY, pointJacZ ) in 
+      let scalarX = gsub result (size 0) (size 32) in 
+      let scalarY = gsub result (size 32) (size 32) in 
+  
+      as_seq h1 scalarX == nat_to_bytes_be 32 xN /\
+      as_seq h1 scalarY == nat_to_bytes_be 32 yN
+    )
+  )
+
+let scalarMultRaw result pubKey scalar =
+  push_frame();
+  
+  let resultBufferFelem = create (size 12) (u64 0) in
+  let publicKeyAsFelem = create (size 12) (u64 0) in
+  let tempBuffer = create (size 100) (u64 0) in
+    
+  toFormPoint pubKey publicKeyAsFelem; 
+  (* with normalisation *)
+  scalarMultiplication publicKeyAsFelem resultBufferFelem scalar tempBuffer;
+  fromFormPoint resultBufferFelem result;
+
+  pop_frame()
+
+
+inline_for_extraction noextract
+val ecdsa_verification_point_operations: result: lbuffer uint8 (size 32) -> publicKey: lbuffer uint8 (size 64) -> 
+  u1: lbuffer uint8 (size 32) -> u2: lbuffer uint8 (size 32) ->
+  Stack bool 
+  (requires fun h -> live h result /\ live h publicKey /\ live h u1 /\ live h u2 /\
+    LowStar.Monotonic.Buffer.all_disjoint [loc result; loc publicKey; loc u1; loc u2] /\ (
+    let publicKeyX = nat_from_bytes_be (as_seq h (gsub publicKey (size 0) (size 32))) in
+    let publicKeyY = nat_from_bytes_be (as_seq h (gsub publicKey (size 32) (size 32))) in 
+    publicKeyX < prime256 /\ publicKeyY < prime256 ))
+  (ensures fun h0 r h1 -> modifies (loc result) h0 h1 /\ (
+    let pointScalarXSeq = nat_from_bytes_be (as_seq h0 (gsub publicKey (size 0) (size 32))) in 
+    let pointScalarYSeq = nat_from_bytes_be (as_seq h0 (gsub publicKey (size 32) (size 32))) in 
+    let pubJac = toJacobianCoordinates (pointScalarXSeq, pointScalarYSeq) in 
+    let pointAtInfinity = (0, 0, 0) in
+    let u1D, _ = montgomery_ladder_spec (as_seq h0 u1) (pointAtInfinity, basePoint) in
+    let u2D, _ = montgomery_ladder_spec (as_seq h0 u2) (pointAtInfinity, pubJac) in
+    let sumD = if  _norm u1D =  _norm u2D then  _point_double u1D else  _point_add u1D u2D in 
+    let pointNorm = _norm sumD in
+    let (xResult, yResult, zResult) = pointNorm in
+    r == not (Spec.P256.isPointAtInfinity pointNorm) /\
+    as_seq h1 result == nat_to_bytes_be 32  (xResult % prime_p256_order)))
+
+
+let ecdsa_verification_point_operations result publicKey u1 u2 = 
+  push_frame();
+    let tempBuffer = create (size 100) (u64 0) in  
+    let publicKeyAsFelem = create (size 12) (u64 0) in 
+    let resultFelem = create (size 4) (u64 0) in 
+
+  toFormPoint publicKey publicKeyAsFelem;
+  let r = Hacl.Impl.ECDSA.P256.Verification.Agile.ecdsa_verification_step5 resultFelem publicKeyAsFelem u1 u2 tempBuffer in 
+  _fromForm resultFelem result;
+  
+  pop_frame();
+  r
